src/cbor/spec/raw/CBOR.Spec.Raw.Valid2.fsti
@@ -1,0 +1,85 @@
+module CBOR.Spec.Raw.Valid2
+include CBOR.Spec.Raw.Base
+open CBOR.Spec.Util
+
+val valid
+  (data_model: (raw_data_item -> raw_data_item -> bool))
+  (x: raw_data_item)
+: Tot bool
+
+val equiv
+  (data_model: (raw_data_item -> raw_data_item -> bool))
+  (x1 x2: raw_data_item)
+: Tot bool
+
+val valid_eq
+  (data_model: (raw_data_item -> raw_data_item -> bool))
+  (x: raw_data_item)
+: Lemma
+  (ensures (valid data_model x == (
+    match x with
+    | Array _ v -> List.Tot.for_all (valid data_model) v
+    | Tagged _ v -> valid data_model v
+    | Map _ v ->
+      List.Tot.for_all (valid data_model) (List.Tot.map fst v) &&
+      List.Tot.for_all (valid data_model) (List.Tot.map snd v) &&
+      not (list_no_setoid_repeats (equiv data_model) (List.Tot.map fst v))
+    | _ -> true
+  )))
+
+val equiv_eq
+  (data_model: (raw_data_item -> raw_data_item -> bool))
+  (x1 x2: raw_data_item)
+: Lemma
+  (ensures equiv data_model x1 x2 == (
+  if data_model x1 x2
+  then true
+  else if x1 = x2
+  then true
+  else
+    valid data_model x1 && valid data_model x2 &&
+    begin match x1, x2 with
+    | Array _ v1, Array _ v2 ->
+      list_for_all2 (equiv data_model) v1 v2
+    | Map _ v1, Map _ v2 ->
+      List.Tot.for_all (setoid_assoc_eq (equiv data_model) (equiv data_model) v2) v1 &&
+      List.Tot.for_all (setoid_assoc_eq (equiv data_model) (equiv data_model) v1) v2
+    | Tagged tag1 v1, Tagged tag2 v2 ->
+      tag1.value = tag2.value &&
+      equiv data_model v1 v2
+    | Int64 ty1 v1, Int64 ty2 v2 ->
+      ty1 = ty2 && v1.value = v2.value
+    | String ty1 _ v1, String ty2 _ v2 ->
+      ty1 = ty2 && v1 = v2
+    | _ -> false
+    end
+  ))
+
+val equiv_refl
+  (data_model: (raw_data_item -> raw_data_item -> bool))
+  (x1: raw_data_item)
+: Lemma
+  (ensures equiv data_model x1 x1)
+
+val equiv_sym
+  (data_model: (raw_data_item -> raw_data_item -> bool) {
+    forall x1 x2 . data_model x1 x2 == data_model x2 x1
+  })
+  (x1 x2: raw_data_item)
+: Lemma
+  (ensures equiv data_model x1 x2 == equiv data_model x2 x1)
+
+let valid_item
+  (data_model: (raw_data_item -> raw_data_item -> bool))
+  (x: raw_data_item)
+: Tot bool
+=   match x with
+    | Map _ v ->
+      not (list_no_setoid_repeats (equiv data_model) (List.Tot.map fst v))
+    | _ -> true
+
+val valid_eq'
+  (data_model: (raw_data_item -> raw_data_item -> bool))
+  (x: raw_data_item)
+: Lemma
+  (ensures (valid data_model x == holds_on_raw_data_item (valid_item data_model) x))
